BoC/Model.lean
@@ -2,38 +2,52 @@ import Mathlib.Logic.Relation
 import BoC.Common
 import BoC.History
 
--- Program order relation
-def po_relation (events : Set Event) : Event → Event → Prop
-| .Run bid1, .Spawn bid2 =>
-    .Run bid1 ∈ events ∧
-    .Spawn bid2 ∈ events
-| .Spawn bid1, .Spawn bid2 =>
-    .Spawn bid1 ∈ events ∧
-    .Spawn bid2 ∈ events
-| .Spawn bid1, .Commit bid2 =>
-    .Spawn bid1 ∈ events ∧
-    .Commit bid2 ∈ events
-| _, _ => False
-
--- Coherence order relation
-def co_relation (events : Set Event) : Event → Event → Cown → Prop
-| .Commit bid1, .Run bid2, _ =>
-    .Commit bid1 ∈ events ∧
-    .Run bid2 ∈ events
-| _, _, _ => False
-
 -- A model is a set of events along with a given program order, coherence order
 -- and a disjointness relation on cown sets
 structure Model where
   mk ::
   (events : Set Event)
-  (po : Event -> Event -> Prop := po_relation events)
-  (co : Event → Event → Cown → Prop := co_relation events)
+  (po : Event → Event → Prop)
+  (co : Event → Event → Cown → Prop)
   -- (disj : Set Cown → Set Cown → Prop)
+
+def wf_po_relation (events : Set Event) (po : Event → Event → Prop) : Prop :=
+  -- po only relates known events
+  (∀e1 e2, po e1 e2 → e1 ∈ events ∧ e2 ∈ events)
+  ∧
+  -- po relates run/spawn, spawn/spawn, and spawn/commit events
+  (∀e1 e2, po e1 e2 → match e1, e2 with
+                      | .Run _, .Spawn _
+                      | .Spawn _, .Spawn _
+                      | .Spawn _, .Complete _ => True
+                      | _, _ => False)
+  ∧
+  -- po uniquely determines its predecessors and successors (po is a bijection?)
+  (∀e1 e2 e3, po e1 e3 → po e2 e3 → e1 = e2) ∧
+  (∀e1 e2 e3, po e1 e2 → po e1 e3 → e2 = e3)
+  ∧
+  -- All events are preceeded by a Run event
+  (∀e1 e2, po e1 e2 → ∃bid, (po*) (.Run bid) e1)
+  ∧
+  -- A completion event must finish the same behaviour that was started
+  (∀bid1 bid2, (po+) (.Run bid1) (.Complete bid2) → bid1 = bid2)
+
+def wf_co_relation (events : Set Event) (co : Event → Event → Cown → Prop) : Prop :=
+  -- co only relates known events
+  (∀e1 e2 c, co e1 e2 c → e1 ∈ events ∧ e2 ∈ events)
+  ∧
+  -- co relates commit/run events
+  (∀e1 e2 c, co e1 e2 c → match e1, e2 with
+                          | .Complete _, .Run _ => True
+                          | _, _ => False)
+  ∧
+  -- co uniquely determines its predecessors and successors (co is a bijection?)
+  (∀e1 e2 e3 c, co e1 e3 c → co e2 e3 c → e1 = e2) ∧
+  (∀e1 e2 e3 c, co e1 e2 c → co e1 e3 c → e2 = e3)
 
 -- From a model, we can derive a run relation which relates a spawn event of a
 -- behaviour to the corresponding run event
-def derived_run (m : Model) : Event → Event → Prop
+def derived_run_relation (m : Model) : Event → Event → Prop
 | .Spawn bid, .Run bid' =>
     bid = bid' ∧
     .Spawn bid ∈ m.events ∧
@@ -42,58 +56,49 @@ def derived_run (m : Model) : Event → Event → Prop
 
 -- From a model we can derive a happens-before relation which relates a commit
 -- with all the runs that happened after it
-def derived_hb (m : Model) : Event → Event → Prop
-| .Commit bid1, .Run bid2 =>
-  let r := derived_run m;
+def derived_hb_relation (m : Model) : Event → Event → Prop
+| .Complete bid1, .Run bid2 =>
+  let r := derived_run_relation m;
   let co' := fun e1 e2 => ∃c, m.co e1 e2 c;
-  let cowns bid := {c | (∃e, m.co e (.Run bid) c) ∨ (∃e, m.co (.Commit bid) e c)};
+  let cowns bid := {c | (∃e, m.co e (.Run bid) c) ∨ (∃e, m.co (.Complete bid) e c)};
   let conflict bid1 bid2 := (cowns bid1) ∩ (cowns bid2) ≠ ∅;
   ∃bid_origin bid_spawn,
-    (r ∘ (m.po+)) (.Spawn bid_origin) (.Commit bid1) ∧
+    (r ∘ (m.po+)) (.Spawn bid_origin) (.Complete bid1) ∧
     ((m.po ∪ co' ∪ r)+) (.Spawn bid_origin) (.Spawn bid_spawn) ∧
     r (.Spawn bid_spawn) (.Run bid2) ∧
     conflict bid1 bid2 ∧
     bid1 ≠ bid2
 | _, _ => False
 
--- TODO: Break out well-formed po and co definitions
--- TODO: Run events are minimal elements in po
 -- Well-formedness conditions for a model
 def Model.wf : Model → Prop
 | m@⟨events, po, co⟩ =>
-  let r := derived_run m;
-  let hb := derived_hb m;
+  -- Derived relations
+  let r := derived_run_relation m;
+  let hb := derived_hb_relation m;
   let co_k c := fun e1 e2 => co e1 e2 c;
   let co' := fun e1 e2 => ∃c, co e1 e2 c;
-  /-1: relations only mention known events -/
-  (∀e1 e2, po e1 e2 → e1 ∈ events ∧ e2 ∈ events) ∧
-  (∀e1 e2 c, co e1 e2 c → e1 ∈ events ∧ e2 ∈ events) ∧
-  /-2: The transitive closure of po_co_r is acyclic -/
+  wf_po_relation events po ∧
+  wf_co_relation events co ∧
+  -- The transitive closure of po ∪ co ∪ r is acyclic
   (∀e1 e2, ((po ∪ co' ∪ r)+) e1 e2 → e1 ≠ e2) ∧
-  /-3: A commit event must finish the same behaviour that was started -/
-  (∀bid1 bid2, (po+) (.Run bid1) (.Commit bid2) → bid1 = bid2) ∧
-  /-4: po uniquely determines its predecessors -/
-  (∀e1 e2 e3, po e1 e3 → po e2 e3 → e1 = e2) ∧
-  /-5: po uniquely determines its successors -/
-  (∀e1 e2 e3, po e1 e2 → po e1 e3 → e2 = e3) ∧
-  /-6: co uniquely determines its predecessors -/
-  (∀e1 e2 e3 c, co e1 e3 c → co e2 e3 c → e1 = e2) ∧
-  /-7: co uniquely determines its successors -/
-  (∀e1 e2 e3 c, co e1 e2 c → co e1 e3 c → e2 = e3) ∧
-  /-8: co creates a single causal order path for any given cown -/
+  -- co creates a single causal order path for any given cown
   (∀e1 e2 e3 e4 c,
     e1 ≠ e3 →
     e2 ≠ e4 →
     co e1 e2 c →
     co e3 e4 c →
     ((po ∪ co_k c)+) e2 e3 ∨ ((po ∪ co_k c)+) e4 e1) ∧
-  /-9: The transitive closure of po_co_hb is acyclic -/
+  -- The transitive closure of po_co_hb is acyclic
   (∀e1 e2, ((po ∪ co' ∪ hb)+) e1 e2 → e1 ≠ e2)
-  -- TODO: Program order events must start with a Run event
-  -- TODO: Coherence order events must start with a Commit event
 
-  -- TODO: Distinguish between partial and complete models
-
+def Model.complete : Model → Prop
+| ⟨events, po, _⟩ =>
+  -- Every run event has a corresponding complete event
+  (∀bid, .Run bid ∈ events → (po+) (.Run bid) (.Complete bid))
+  ∧
+  -- Every spawn event has a corresponding run event
+  (∀bid, .Spawn bid ∈ events → .Run bid ∈ events)
 
 -- TODO: def model_from_history
 -- TODO: ⊢ H → History.complete H → Model.wf (model_from_history H)
